disk-betree/ImplMarshalling.i.dfy
@@ -110,8 +110,9 @@ module ImplMarshalling {
 
   method ValToIndirectionTable(v: V) returns (s : Option<ImplState.MutIndirectionTable>)
   requires IMM.valToIndirectionTable.requires(v)
-  ensures MapOption(s, (x: ImplState.MutIndirectionTable) reads x => x.I()) == IMM.valToIndirectionTable(v)
+  ensures s.None? ==> IMM.valToIndirectionTable(v).None?
   ensures s.Some? ==> s.value.Inv()
+  ensures s.Some? ==> IMM.valToIndirectionTable(v) == Some(s.value.I())
   {
     var res := ValToLocsAndSuccs(v.a);
     match res {
@@ -626,16 +627,15 @@ module ImplMarshalling {
         assert forall r | r in mutMap.I().contents :: r in IM.IIndirectionTable(sector.indirectionTable.I()).locs
             ==> mutMap.I().contents[r].0.Some? && BC.ValidLocationForNode(mutMap.I().contents[r].0.value);
         if mutMap.Count < 0x2000_0000_0000_0000 {
-          // TODO this probably warrants a new invariant, or may leverage the weights branch, see TODO in BlockCache
-
           var a: array<V> := new V[mutMap.Count as uint64];
           var it := mutMap.IterStart();
           var i := 0;
           ghost var partial := map[];
           while it.next.Some?
+          invariant 0 <= i <= a.Length
           invariant MutableMapModel.WFIter(mutMap.I(), it);
-          invariant forall j | j < i :: ValidVal(a[j])
-          invariant forall j | j < i :: ValInGrammar(a[j], GTuple([GUint64, GUint64, GUint64, GUint64Array]))
+          invariant forall j | 0 <= j < i :: ValidVal(a[j])
+          invariant forall j | 0 <= j < i :: ValInGrammar(a[j], GTuple([GUint64, GUint64, GUint64, GUint64Array]))
           // NOALIAS/CONST table doesn't need to be mutable, if we could say so we wouldn't need this
           invariant IMM.valToLocsAndSuccs(a[..i]).Some?
           invariant IMM.valToLocsAndSuccs(a[..i]).value.contents == partial
@@ -645,12 +645,19 @@ module ImplMarshalling {
           invariant forall r | r in partial :: r in mutMap.I().contents && partial[r] == mutMap.I().contents[r]
           // NOALIAS/CONST mutMap doesn't need to be mutable, if we could say so we wouldn't need this
           invariant mutMap.I().contents == old(mutMap.I().contents)
+          decreases it.decreaser
           {
             var (ref, locOptGraph: (Option<LBAType.Location>, seq<Reference>)) := it.next.value;
             // NOTE: deconstructing in two steps to work around c# translation bug
             var (locOpt, graph) := locOptGraph;
             var loc := locOpt.value;
             var childrenVal := VUint64Array(graph);
+
+            MutableMapModel.LemmaIterIndexLtCount(mutMap.I(), it);
+
+            // TODO this probably warrants a new invariant, or may leverage the weights branch, see TODO in BlockCache
+            assume |graph| < 0x1_0000_0000_0000_0000;
+            assert ValidVal(VTuple([IMM.refToVal(ref), IMM.lbaToVal(loc.addr), VUint64(loc.len), childrenVal]));
 
             // == mutation ==
             partial := partial[ref := (locOpt, graph)];
